LeanBoogie/Effect/Mem.lean
@@ -3,7 +3,7 @@ import LeanBoogie.ConTy
 import Mathlib.Data.Real.Basic
 
 namespace LeanBoogie
-open ITree (HasEff)
+open ITree (HasEff trigger Handler None)
 
 /-
   # Memory (Effects) in Boogie
@@ -16,23 +16,45 @@ open ITree (HasEff)
 inductive Mem (Γ : Con) : Type -> Type where
 | rd : Var Γ A          -> Mem Γ A
 | wr : Var Γ A -> TyA A -> Mem Γ Unit
+-- | swap : List ((A : Ty) × Var Γ A) -> List ((A : Ty) × Var Γ A) -> Mem Γ Unit
 
-def Mem.read  (v : Var Γ A)           : ITree (Mem Γ) A    := .vis (.rd v    ) .ret
-def Mem.write (v : Var Γ A) (val : A) : ITree (Mem Γ) Unit := .vis (.wr v val) .ret
+def Mem.read  (v : Var Γ A)           : ITree (Mem Γ) A    := trigger (.rd v)
+def Mem.write (v : Var Γ A) (val : A) : ITree (Mem Γ) Unit := trigger (.wr v val)
+
 /-- Apply a pure function to a variable. E.g. `Mem.update x (· + 10)`. -/
 abbrev Mem.update (v : Var Γ A) (f : A -> A) : ITree (Mem Γ) Unit := do
   let val <- read v
   write v (f val)
 
-def Mem.read'  (v : Var Γ A)           : ITree (E & Mem Γ) A    := .vis (Mem.rd v    ) .ret
-def Mem.write' (v : Var Γ A) (val : A) : ITree (E & Mem Γ) Unit := .vis (Mem.wr v val) .ret
+-- def Mem.read'  (v : Var Γ A)           : ITree (E & Mem Γ) A    := .vis (Mem.rd v    ) .ret
+-- def Mem.write' (v : Var Γ A) (val : A) : ITree (E & Mem Γ) Unit := .vis (Mem.wr v val) .ret
+-- -- the most general form is like this, with `HasEff`:
+-- def Mem.read''  [HasEff (Mem Γ) E] (v : Var Γ A)           : ITree E A    := .vis (Mem.rd v    ) .ret
+-- def Mem.write'' [HasEff (Mem Γ) E] (v : Var Γ A) (val : A) : ITree E Unit := .vis (Mem.wr v val) .ret
 
--- the most general form is like this, with `HasEff`:
-def Mem.read''  [HasEff (Mem Γ) E] (v : Var Γ A)           : ITree E A    := .vis (Mem.rd v    ) .ret
-def Mem.write'' [HasEff (Mem Γ) E] (v : Var Γ A) (val : A) : ITree E Unit := .vis (Mem.wr v val) .ret
+-- def Mem.merge : ITree (Mem Γ & Mem Δ) A -> ITree (Mem (Γ ++ Δ)) A := sorry
 
-def Mem.merge : ITree (Mem Γ & Mem Δ) A -> ITree (Mem (Γ ++ Δ)) A := sorry
-def Mem.split : ITree (Mem (Γ ++ Δ)) A -> ITree (Mem Γ & Mem Δ) A := sorry
+-- def Mem.handle_split : Handler (Mem (Γ ++ Δ)) (ITree)
+def Mem.split : Mem (Γ ++ Δ) A -> (Mem Γ & Mem Δ) A
+| .rd v => match v.split with
+  | .inl v => .left (.rd v)
+  | .inr v => .right (.rd v)
+| .wr v val => match v.split with
+  | .inl v => .left (.wr v val)
+  | .inr v => .right (.wr v val)
+
+instance : HasEff (Mem (Γ ++ Δ)) (Mem Γ & Mem Δ) where
+  inj := Mem.split
+
+instance : HasEff (Mem []) None where inj e := nomatch e
+instance : HasEff (Mem []) ∅ where inj e := nomatch e
+instance : HasEff (Mem []) 0 where inj e := nomatch e
+
+-- instance : HasEff (Mem Γ & Mem Δ) (Mem (Γ ++ Δ)) where
+--   inj := Mem.merge
+
+-- def Mem.split : ITree (Mem (Γ ++ Δ)) A -> ITree (Mem Γ & Mem Δ) A := by
+--   sorry
 
 
 private def Γ : Con := [.int, .bv 32, .bool ~> .int]
