LeanBoogie/State.lean
@@ -1,8 +1,10 @@
 import LeanBoogie.Effect.Mem
 import LeanBoogie.Notation.Iter
+import LeanBoogie.ITree.Effect
 import LeanBoogie.ConTy
 
 namespace LeanBoogie
+open ITree
 
 /-
   The file `Mem.lean` only defines the `Mem` effect, but lacks any interpretation.
@@ -18,6 +20,7 @@ namespace LeanBoogie
   # The state monad
 -/
 
+
 def State.read [Monad M] (v : Var Γ A) : StateT Γ M A := fun γ => return (γ.get v, γ)
 def State.write [Monad M] (v : Var Γ A) (val : A) : StateT Γ M PUnit := fun γ => return (.unit, γ.set v val)
 
@@ -32,6 +35,45 @@ def State.iter [Monad M] [Iter M] /- {Γ : Con} -/ (f : A -> StateT Γ M (A ⊕ 
 
 instance [Monad M] [Iter M] : Iter (StateT Γ M) := ⟨State.iter⟩
 
+
+
+section
+/-
+  # Interpreting
+-/
+
+variable {M : Type _ -> Type _} [Monad M]
+variable [Iter M]
+
+/-- We can interpret memory events into any monad, with our state monad on top. This is actually
+  a family of handlers, one for every monad `M`. Although `M` is usually another `ITree _`. -/
+def State.handler [Monad M] : Handler (Mem Γ) (StateT Γ M)
+| _, .rd v => State.read v
+| _, .wr v val => State.write v val
+
+theorem State.interp_read {v : Var Γ A} : interp State.handler (Mem.read v) = State.read (M := M) v := by
+  rw [Mem.read, interp_trigger]; rfl
+
+theorem State.interp_write {v : Var Γ A} : interp State.handler (Mem.write v val) = (State.write (M := M) v val) := by
+  rw [Mem.write, interp_trigger]; rfl
+end
+
+/-- Given an ITree which may refer to default-initialized local vars `L`, parameters `P`,
+  obtain a `P -> ITree (Mem G) R`. -/
+def runProc {P L : Con} {R : Type} (t : ITree (Mem (L ++ P)) R) (p : P) : ITree (Mem []) R :=
+  let tL : StateT (L ++ P) (ITree (Mem [])) R := interp State.handler t
+  Prod.fst <$> (tL ((default : L) ++ p))
+
+#synth MonadLiftT (ITree (Mem ?Γ)) (StateT (ConA [?A]) (ITree (Mem ?Γ)) )
+
+def runRes {A : Ty} (t : ITree (Mem ([A] ++ Γ)) Unit) (a : A) : ITree (Mem Γ) A :=
+  let hleft  : Handler (Mem [A]        ) (StateT [A] (ITree (Mem Γ))) := State.handler
+  let hright : Handler (          Mem Γ) (StateT [A] (ITree (Mem Γ))) := fun _ e => liftM (trigger e) -- this liftM feels dirty, maybe there's a better way
+  let h      : Handler (Mem [A] & Mem Γ) (StateT [A] (ITree (Mem Γ))) := Handler.case hleft hright
+  let t :             ITree (Mem [A] & Mem Γ)  Unit             := embed t
+  let t : ConA [A] -> ITree (          Mem Γ) (Unit × ConA [A]) := interp h t
+  (Prod.fst ∘ Prod.snd) <$> t (a, ())
+
 /-
   ## Equational reasoning for our state monad
 
@@ -42,7 +84,6 @@ instance [Monad M] [Iter M] : Iter (StateT Γ M) := ⟨State.iter⟩
   * A lot of theorems about how our state behaves are proven in `Types.lean`, usually named `ConA_*`.
 -/
 
-
 theorem State.ite_push_state [Decidable c] {t e : StateT Γ M A}
   : (if c then t else e) σ = (if c then t σ else e σ)
   := by split <;> simp_all only
@@ -50,71 +91,3 @@ theorem State.ite_push_state [Decidable c] {t e : StateT Γ M A}
 theorem State.bind_push_state [Monad M] {a : StateT Γ M A} {b : A -> StateT Γ M B}
   : (a >>= b) σ = (a σ >>= fun res => b res.fst res.snd)
   := rfl
-
-
-
-/-
-  # Interpreting
--/
-
-def handle [Monad M] : Mem Γ Ans -> StateT Γ M Ans
-| .rd v => State.read v
-| .wr v val => State.write v val
-
-def interp (tm : ITree (Mem Γ) A) : StateT Γ (ITree ∅) A := fun s₀ =>
-  ITree.corec (fun ⟨tm, s⟩ =>
-    match tm.dest with
-    | .ret (.up a) => .ret (.up (a, s))
-    | .tau t => .tau (t, s)
-    | .vis ⟨Ans, .up ((e : Mem Γ Ans)), (k : ULift Ans -> ITree (Mem Γ) A)⟩ =>
-      -- would be nice to use `handle` here instead of the match
-      -- let m : StateT Γ (ITree ∅) Ans := handle e
-      match e with
-      | .rd v => .tau ⟨k (.up (s.get v)), s⟩
-      | .wr v val => .tau ⟨k (.up ()), s.set v val⟩
-  ) (tm, s₀)
-
-def interp' {E : Type -> Type} (tm : ITree (Mem Γ & E) A) : StateT Γ (ITree E) A := fun s₀ =>
-  ITree.corec (fun ⟨tm, s⟩ =>
-    match tm.dest with
-    | .ret (.up a) => .ret (.up (a, s))
-    | .tau t => .tau (t, s)
-    | .vis ⟨Ans, .up (.right (e : E Ans    )), k⟩ => .vis ⟨Ans, .up e, fun ans => ⟨k ans, s⟩⟩ -- don't interpret the rest of the effects.
-    | .vis ⟨Ans, .up (.left  (e : Mem Γ Ans)), (k : ULift Ans -> ITree (Mem Γ & E) A)⟩ =>
-      match e with
-      | .rd v => .tau ⟨k (.up (s.get v)), s⟩
-      | .wr v val => .tau ⟨k (.up ()), s.set v val⟩
-  ) (tm, s₀)
-
--- Ideally we want something as general as this:
--- def interp'' {E : Type -> Type} [inst : HasEff (Mem Γ) E] (tm : ITree E A) : StateT Γ (ITree inst.Strip) A := fun s₀ =>
---   ITree.corec (fun ⟨tm, s⟩ =>
---     match tm.dest with
---     | .ret (.up a) => .ret (.up (a, s))
---     | .tau t => .tau (t, s)
---     | .vis ⟨Ans, .up ((e : E Ans    )), k⟩ =>
---       inst.elim (fun e =>
---         match e with
---         | .rd v => .tau ⟨k (.up (s.get v)), s⟩
---         | .wr v val => .tau ⟨k (.up ()), s.set v val⟩
---       ) (fun e => .vis e k) e
---   ) (tm, s₀)
-
-theorem interp_pure : interp (pure a : ITree (Mem Γ) A) = pure a := sorry
-
-theorem interp_bind {ta : ITree (Mem Γ) A} {tb : A -> ITree (Mem Γ) B}
-  : interp (ta >>= tb) = (interp ta) >>= (fun a => interp (tb a))
-  := sorry
-
--- /-- Convenience mix of `interp_bind` and `bind_state_pull`. -/
-theorem interp_bind_pull {ta : ITree (Mem Γ) A} {tb : A -> ITree (Mem Γ) B}
-  : interp (bind ta tb) s = bind (interp ta s) (fun x => interp (tb x.1) x.2)
-  := sorry
-
-theorem interp_iter {f : A -> ITree (Mem Γ) (A ⊕ B)} {a₀ : A}
-  : interp (iter f a₀) = iter (fun (a : A) => interp (f a)) a₀
-  := sorry
-
-theorem interp_read {v : Var Γ A} : interp (Mem.read v) = State.read v := sorry
-theorem interp_write {v : Var Γ A} : interp (Mem.write v val) = (State.write v val) := sorry
-theorem interp_ite [Decidable φ] : interp (if φ then t else e) = (if φ then interp t else interp e) := sorry
